Introduce synpty

nola/examples/logic/synty.v
@@ -3,9 +3,9 @@
 From nola.iris Require Export prophecy.
 
 (** Syntactic type *)
-Inductive nsynty := Empty_setₛ | unitₛ | boolₛ | natₛ | Zₛ | Propₛ
-| optionₛ (X : nsynty) | listₛ (X : nsynty) | prodₛ (X Y : nsynty)
-| sumₛ (X Y : nsynty) | funₛ (X Y : nsynty).
+Inductive nsynty := Empty_setₛ | unitₛ | boolₛ | natₛ | Zₛ | Propₛ | nsyntyₛ
+| aprvarₛ | prvarₛ (X : nsynty) | optionₛ (X : nsynty) | listₛ (X : nsynty)
+| prodₛ (X Y : nsynty) | sumₛ (X Y : nsynty) | funₛ (X Y : nsynty).
 Implicit Type (X Y : nsynty).
 
 Declare Scope nsynty_scope.
@@ -15,36 +15,49 @@ Notation "()" := unitₛ : nsynty_scope.
 Infix "*" := prodₛ : nsynty_scope. Infix "+" := sumₛ : nsynty_scope.
 Infix "→" := funₛ : nsynty_scope.
 
+(** Decidable equality *)
+#[export] Instance nsynty_eq_dec : EqDecision nsynty.
+Proof. solve_decision. Defined.
+
+(** [nsynty] is inhabited *)
+#[export] Instance nsynty_inhabited : Inhabited nsynty := populate Empty_setₛ.
+
+(** Decidable inhabitedness *)
+Fixpoint nsynty_inhab X : bool :=
+  match X with
+  | Empty_setₛ => false | prvarₛ X => nsynty_inhab X
+  | prodₛ X Y => nsynty_inhab X && nsynty_inhab Y
+  | sumₛ X Y => nsynty_inhab X || nsynty_inhab Y
+  | funₛ X Y => negb (nsynty_inhab X) || nsynty_inhab Y
+  | _ => true
+  end.
+
+(** Syntactic pre-type structure *)
+Canonical nsynty_synpty : synpty :=
+  {| synpty_car := nsynty; synpty_inhab := nsynty_inhab; |}.
+
+Notation aprvarn := (aprvar nsynty).
+
 (** Interpret [nsynty] as a type *)
 Fixpoint nsynty_ty (X : nsynty) : Type :=
   match X with
   | Empty_setₛ => Empty_set | unitₛ => () | boolₛ => bool | natₛ => nat
-  | Zₛ => Z | Propₛ => Prop | optionₛ X => option (nsynty_ty X)
+  | Zₛ => Z | Propₛ => Prop | nsyntyₛ => nsynty | aprvarₛ => aprvarn
+  | prvarₛ X => prvar X | optionₛ X => option (nsynty_ty X)
   | listₛ X => list (nsynty_ty X) | prodₛ X Y => nsynty_ty X * nsynty_ty Y
   | sumₛ X Y => nsynty_ty X + nsynty_ty Y
   | funₛ X Y => nsynty_ty X → nsynty_ty Y
   end.
 Coercion nsynty_ty: nsynty >-> Sortclass.
 
-(** Decidable equality *)
-#[export] Instance nsynty_eq_dec : EqDecision nsynty.
-Proof. solve_decision. Defined.
-
-(** Decidable inhabitedness *)
-
-Fixpoint nsynty_inhab X : bool :=
-  match X with
-  | Empty_setₛ => false | prodₛ X Y => nsynty_inhab X && nsynty_inhab Y
-  | sumₛ X Y => nsynty_inhab X || nsynty_inhab Y
-  | funₛ X Y => negb (nsynty_inhab X) || nsynty_inhab Y
-  | _ => true
-  end.
-
+(** [nsynty_inhab] is equivalent to inhabitance *)
 Local Lemma of_either_nsynty_inhab {X} :
   (nsynty_inhab X → X) * (negb (nsynty_inhab X) → X → False).
 Proof.
   move: X. fix FIX 1. move=> X. split.
   - case: X=>//=; try by (move=> *; exact inhabitant).
+    + move=> ?. by apply (aprvar_by_inhab unitₛ).
+    + move=> X h. exact (prvar_by_inhab X h).
     + move=> ?? /andb_True[??]. constructor; by apply FIX.
     + move=> X ?. case eq: (nsynty_inhab X)=>/= H.
       * apply inl, FIX. by rewrite eq.
@@ -52,8 +65,9 @@ Proof.
     + move=> X ?. case eq: (nsynty_inhab X)=>/= ??; [by apply FIX|].
       exfalso. eapply FIX; [|done]. by rewrite eq.
   - case: X=>//=.
+    + move=> X /negb_True. apply (prvar_neg_inhab X).
     + move=> X ?. rewrite negb_andb.
-      case eq: (nsynty_inhab X)=>/= ?[a?]; [by eapply FIX|].
+      case eq: (nsynty_inhab X)=>/= ?[a b]; [by eapply FIX|].
       eapply FIX; [|apply a]. by rewrite eq.
     + move=> ??. by rewrite negb_orb=> /andb_True[??] [a|b];
       eapply FIX; [|apply a| |apply b].
@@ -64,25 +78,22 @@ Lemma of_nsynty_inhab {X} : nsynty_inhab X → X.
 Proof. apply of_either_nsynty_inhab. Qed.
 Lemma of_neg_nsynty_inhab {X} : negb (nsynty_inhab X) → X → False.
 Proof. apply of_either_nsynty_inhab. Qed.
-Lemma to_nsynty_inhab {X} (x: X) : nsynty_inhab X.
+Lemma to_nsynty_inhab {X} (x : X) : nsynty_inhab X.
 Proof.
   case eq: (nsynty_inhab X); [done|]. exfalso.
   eapply of_neg_nsynty_inhab; [|done]. by rewrite eq.
 Qed.
-Lemma to_neg_nsynty_inhab {X} (f: X → False) : negb (nsynty_inhab X).
+Lemma to_neg_nsynty_inhab {X} (f : X → False) : negb (nsynty_inhab X).
 Proof.
   case eq: (nsynty_inhab X); [|done]. exfalso. apply f, of_nsynty_inhab.
   by rewrite eq.
 Qed.
 
-(** [nsynty] is [synty] *)
-Program Canonical nsynty_synty : synty := {|
-  synty_car := nsynty; synty_ty := nsynty_ty; synty_inhab := nsynty_inhab;
-|}.
+(** Syntactic type structure *)
+Program Canonical nsynty_synty : synty :=
+  {| synty_pty := nsynty_synpty; synty_ty := nsynty_ty; |}.
 Next Obligation. by move=> ? /of_nsynty_inhab. Qed.
 Next Obligation. by move=> ? /to_nsynty_inhab. Qed.
 
-Notation prvarn := (prvar nsynty).
-Notation aprvarn := (aprvar nsynty).
 Notation proph_asnn := (proph_asn nsynty).
 Notation prophn A := (proph nsynty A).
